From20To30/Expr.v
@@ -1,0 +1,1223 @@
+From Coq Require Import String ZArith NArith Eqdep_dec Lia.
+
+From Coq Require PropExtensionality.
+
+From Vyper Require Import Config Calldag L10.Base.
+From Vyper Require L20.AST L30.AST L20.Interpret L30.Interpret.
+
+From Vyper.From20To30 Require Import Translate Callset FunCtx.
+
+(** The local memory as a dictionary agrees with the local memory as an array.
+  Here's the equation in pseudocode: [
+    locmap[name] = locmem[locvar[name]]
+  ]
+ *)
+Definition VarsAgree {C: VyperConfig}
+                     (varmap: string_map N)
+                     (locmap: string_map uint256)
+                     (locmem: memory)
+:= let _ := string_map_impl in
+   let _ := memory_impl in
+   forall name: string,
+     match Map.lookup locmap name, Map.lookup varmap name with
+     | Some value, Some index => OpenArray.get locmem index = value
+     | None, Some _ | Some _, None => False
+     | None, None => True
+     end.
+
+(* There's no Map.for_all so here it is: *)
+(** All variables in the varmap stay lower then the given bound. *)
+Definition VarsBound {C: VyperConfig}
+                     (varmap: string_map N)
+                     (bound: N)
+:= let _ := string_map_impl in
+   forall name: string,
+     match Map.lookup varmap name with
+     | Some index => (index < bound)%N
+     | None => True
+     end.
+
+Lemma vars_agree_put {C: VyperConfig}
+                     (varmap: string_map N)
+                     (locmap: string_map uint256)
+                     (locmem: memory)
+                     (dst: N)
+                     (value: uint256)
+                     (Agree: VarsAgree varmap locmap locmem)
+                     (Bound: VarsBound varmap dst):
+  let _ := memory_impl in
+  VarsAgree varmap locmap (OpenArray.put locmem dst value).
+Proof.
+unfold VarsAgree in *. intro name.
+unfold VarsBound in Bound.
+assert (A := Agree name).
+assert (B := Bound name).
+destruct (Map.lookup locmap name).
+destruct (Map.lookup varmap name). 2-3: exact A.
+subst.
+rewrite OpenArray.put_ok.
+enough (NE: (dst =? n)%N = false) by now rewrite NE.
+rewrite N.eqb_neq. apply N.lt_neq in B. intro H. symmetry in H. tauto.
+Qed.
+
+Lemma vars_bound_loosen {C: VyperConfig}
+                        {varmap: string_map N}
+                        {old_bound new_bound: N}
+                        (B: VarsBound varmap old_bound)
+                        (L: (old_bound <= new_bound)%N):
+  VarsBound varmap new_bound.
+Proof.
+unfold VarsBound in *.
+intro name. assert (B' := B name). clear B.
+destruct Map.lookup. 2:trivial.
+apply (N.lt_le_trans _ _ _ B' L).
+Qed.
+
+Definition mem_agree {C: VyperConfig} 
+                     (bound exception: N) (mem1 mem2: memory)
+:= let _ := memory_impl in
+   forall n: N,
+     (n < bound)%N
+      ->
+     n <> exception
+      ->
+     OpenArray.get mem1 n = OpenArray.get mem2 n.
+
+Lemma vars_agree_if_mem_agree {C: VyperConfig}
+                              (varmap: string_map N)
+                              (locmap: string_map uint256)
+                              (mem1 mem2: memory)
+                              (Agree1: VarsAgree varmap locmap mem1)
+                              (dst offset: N)
+                              (Bound : VarsBound varmap dst)
+                              (OffsetOk : (dst < offset)%N)
+                              (M: mem_agree offset dst mem1 mem2):
+  VarsAgree varmap locmap mem2.
+Proof.
+unfold VarsAgree in *. intro name.
+unfold mem_agree in M.
+unfold VarsBound in Bound.
+assert (A := Agree1 name).
+assert (B := Bound name).
+destruct (Map.lookup locmap name), (Map.lookup varmap name); try easy.
+rewrite<- M.
+{ exact A. }
+{ apply (N.lt_trans _ _ _ B OffsetOk). }
+apply N.lt_neq. exact B.
+Qed.
+
+Lemma weak_interpret_translated_exprs {C: VyperConfig}
+    {bigger_call_depth_bound smaller_call_depth_bound: nat}
+    (Ebound: bigger_call_depth_bound = S smaller_call_depth_bound)
+    {cd20: L20.Descend.calldag}
+    (builtins: string -> option builtin)
+    (fc: fun_ctx cd20 bigger_call_depth_bound)
+    {cd30: L30.Descend.calldag}
+    (ok: translate_calldag cd20 = inr cd30)
+    {do_call_20: forall
+          (fc': fun_ctx cd20 smaller_call_depth_bound)
+          (world: world_state)
+          (arg_values: list uint256),
+        world_state * expr_result uint256}
+    {do_call_30: forall
+          (fc': fun_ctx cd30 smaller_call_depth_bound)
+          (world: world_state)
+          (arg_values: list uint256),
+        world_state * expr_result uint256}
+    (DoCallOk: forall fc' world arg_values,
+                 do_call_30 (translate_fun_ctx fc' ok) world arg_values
+                  =
+                 do_call_20 fc' world arg_values)
+    (world: world_state)
+    (locmap: string_map uint256)
+    (locmem: memory)
+    {e20: list L20.AST.expr}
+    {s30: L30.AST.stmt}
+    (varmap: string_map N)
+    (offset: N)
+    (Agree: VarsAgree varmap locmap locmem)
+    (Bound: VarsBound varmap offset)
+    (ExprOk: (fix translate_expr_list (varmap: string_map N) (offset: N) (exprs: list AST.expr)
+              {struct exprs}
+              : string + AST.stmt
+              := match exprs with
+                 | nil => inr (AST.SmallStmt AST.Pass)
+                 | (h :: t)%list =>
+                     match translate_expr varmap offset (N.succ offset) h with
+                     | inl err => inl err
+                     | inr h' =>
+                         match translate_expr_list varmap (N.succ offset) t with
+                         | inl err => inl err
+                         | inr t' => inr (AST.Semicolon h' t')
+                         end
+                     end
+                 end) varmap offset e20 = inr s30)
+    (CallOk30: let _ := string_set_impl in 
+       FSet.is_subset (L30.Callset.stmt_callset s30)
+                      (L30.Callset.decl_callset
+                         (fun_decl
+                           (translate_fun_ctx fc ok)))
+       = true)
+    (CallOk20: let _ := string_set_impl in 
+       FSet.is_subset (L20.Callset.expr_list_callset e20)
+                      (L20.Callset.decl_callset
+                        (fun_decl fc))
+       = true)
+    (AllOk: List.Forall
+          (fun e : AST.expr =>
+           forall
+             (CallOk20 : let H := string_set_impl in
+                         FSet.is_subset (L20.Callset.expr_callset e)
+                           (L20.Callset.decl_callset (fun_decl fc)) = true) (world : world_state)
+             (locmem : memory) (dst offset : N),
+           VarsAgree varmap locmap locmem ->
+           VarsBound varmap dst ->
+           (dst < offset)%N ->
+           forall s30 : AST.stmt,
+           translate_expr varmap dst offset e = inr s30 ->
+           forall
+             CallOk30 : let H := string_set_impl in
+                        FSet.is_subset (Callset.stmt_callset s30)
+                          (Callset.decl_callset (fun_decl (translate_fun_ctx fc ok))) = true,
+           let H := string_map_impl in
+           let H0 := memory_impl in
+           let
+           '(world30, mem30, result30) :=
+            Stmt.interpret_stmt Ebound (translate_fun_ctx fc ok) do_call_30 builtins world locmem s30
+              CallOk30 in
+            match L20.Expr.interpret_expr Ebound fc do_call_20 builtins world locmap e CallOk20 with
+            | (world20, ExprSuccess value20) =>
+                result30 = StmtSuccess /\
+                world30 = world20 /\
+                mem_agree offset dst locmem mem30 /\ OpenArray.get mem30 dst = value20
+            | (world20, ExprAbort abort) => result30 = StmtAbort abort
+            end) e20):
+   let _ := string_map_impl in
+   let _ := memory_impl in
+   let '(world30, mem30, result30) := L30.Stmt.interpret_stmt Ebound (translate_fun_ctx fc ok)
+                                                              do_call_30 builtins
+                                                              world locmem s30 CallOk30
+   in let '(world20, result20) :=
+     (fix
+       interpret_expr_list (world0 : world_state) (loc : string_map uint256) 
+                           (e : list AST.expr)
+                           (CallOk : FSet.is_subset (L20.Callset.expr_list_callset e)
+                                       (L20.Callset.decl_callset (fun_decl fc)) = true) {struct e} :
+         world_state * expr_result (list uint256) :=
+         match e as e' return (e = e' -> world_state * expr_result (list uint256)) with
+         | nil => fun _ : e = nil => (world0, ExprSuccess nil)
+         | (h :: t)%list =>
+             fun E : e = (h :: t)%list =>
+             let (world', result_h) :=
+               L20.Expr.interpret_expr Ebound fc do_call_20 builtins world0 loc h
+                 (L20.Callset.callset_descend_head E CallOk) in
+             match result_h with
+             | ExprSuccess x =>
+                 let (world'', result_t) :=
+                   interpret_expr_list world' loc t (L20.Callset.callset_descend_tail E CallOk) in
+                 (world'',
+                 match result_t with
+                 | ExprSuccess y => ExprSuccess (x :: y)%list
+                 | ExprAbort _ => result_t
+                 end)
+             | ExprAbort ab => (world', ExprAbort ab)
+             end
+         end eq_refl) world locmap e20 CallOk20
+   in match result20 with
+      | ExprSuccess values20 => result30 = StmtSuccess
+                                /\
+                               world30 = world20
+                                /\
+                               mem_agree offset offset locmem mem30
+                                /\
+                               List.length values20 = List.length e20
+                                /\
+                               forall i: nat,
+                                 i < List.length e20
+                                  ->
+                                 List.nth_error values20 i
+                                  =
+                                 Some (OpenArray.get mem30 (offset + N.of_nat i)%N)
+      | ExprAbort abort => result30 = StmtAbort abort
+      end.
+Proof.
+cbn. revert world locmem Agree s30 CallOk30 offset Bound ExprOk. induction e20 as [|h]; intros.
+{ inversion ExprOk. now subst. }
+remember (translate_expr varmap offset (N.succ offset) h) as head30.
+destruct head30. { discriminate. }
+
+assert (HeadOk := List.Forall_inv AllOk). cbn in HeadOk.
+assert (TailOk := List.Forall_inv_tail AllOk).
+clear AllOk.
+remember (fix
+            translate_expr_list (varmap : string_map N) (offset : N) (exprs : list AST.expr) {struct
+                                exprs} : string + AST.stmt :=
+              match exprs with
+              | nil => inr (AST.SmallStmt AST.Pass)
+              | (h :: t)%list =>
+                  match translate_expr varmap offset (N.succ offset) h with
+                  | inl err => inl err
+                  | inr h' =>
+                      match translate_expr_list varmap (N.succ offset) t with
+                      | inl err => inl err
+                      | inr t' => inr (AST.Semicolon h' t')
+                      end
+                  end
+              end) as translate_expr_list.
+remember (translate_expr_list varmap (N.succ offset) e20) as tail30.
+destruct tail30 as [|tail30]. { discriminate. }
+inversion ExprOk. subst s30.
+
+cbn.
+assert (H := HeadOk (L20.Callset.callset_descend_head eq_refl CallOk20)
+             world locmem offset (N.succ offset) Agree Bound (N.lt_succ_diag_r offset)
+             s (eq_sym Heqhead30)
+             (L30.Callset.callset_descend_semicolon_left eq_refl CallOk30)).
+clear HeadOk.
+assert (R: (@Callset.callset_descend_semicolon_left C s tail30 (@AST.Semicolon C s tail30)
+          (@Callset.decl_callset C
+             (@fun_decl C (@AST.decl C) (@Callset.decl_callset C) cd30 bigger_call_depth_bound
+                (@translate_fun_ctx C bigger_call_depth_bound cd20 fc cd30 ok)))
+             (@eq_refl (@AST.stmt C) (@AST.Semicolon C s tail30)) CallOk30)
+             =
+         (@Callset.callset_descend_semicolon_left C s tail30 (@AST.Semicolon C s tail30)
+            (@Callset.decl_callset C (@cached_translated_decl C bigger_call_depth_bound cd20 fc cd30 ok))
+            (@eq_refl (@AST.stmt C) (@AST.Semicolon C s tail30)) CallOk30)).
+{ apply PropExtensionality.proof_irrelevance. }
+rewrite<- R. clear R.
+destruct (Stmt.interpret_stmt Ebound (translate_fun_ctx fc ok) do_call_30 builtins world locmem s
+                              (Callset.callset_descend_semicolon_left eq_refl CallOk30))
+      as ((world30, mem30), result30).
+destruct L20.Expr.interpret_expr as (world20, result20).
+destruct result20, result30; try easy.
+destruct H as (_, (H_world, (H_agree, H_value))).
+subst world20 value.
+
+(* head computation succeeded *)
+assert (R:
+        (@Callset.callset_descend_semicolon_right C s tail30 (@AST.Semicolon C s tail30)
+           (@Callset.decl_callset C
+              (@fun_decl C (@AST.decl C) (@Callset.decl_callset C) cd30 bigger_call_depth_bound
+                 (@translate_fun_ctx C bigger_call_depth_bound cd20 fc cd30 ok)))
+           (@eq_refl (@AST.stmt C) (@AST.Semicolon C s tail30)) CallOk30)
+         =
+       (@Callset.callset_descend_semicolon_right C s tail30 (@AST.Semicolon C s tail30)
+          (@Callset.decl_callset C (@cached_translated_decl C bigger_call_depth_bound cd20 fc cd30 ok))
+          (@eq_refl (@AST.stmt C) (@AST.Semicolon C s tail30)) CallOk30)).
+{ apply PropExtensionality.proof_irrelevance. }
+rewrite<- R. clear R.
+
+assert (Agree': VarsAgree varmap locmap mem30).
+{
+  unfold VarsAgree in *. intro name.
+  assert (A := Agree name).
+  assert (B := Bound name).
+  destruct (Map.lookup locmap name); destruct (Map.lookup varmap name); try easy.
+  unfold mem_agree in H_agree.
+  rewrite<- (H_agree n (N.lt_trans _ _ _ B (N.lt_succ_diag_r offset)) (N.lt_neq _ _ B)).
+  exact A.
+}
+
+assert (IH := IHe20 (L20.Callset.callset_descend_tail eq_refl CallOk20) TailOk world30 mem30
+                    Agree'
+                    tail30
+                    (L30.Callset.callset_descend_semicolon_right eq_refl CallOk30)
+                    (N.succ offset) (vars_bound_loosen Bound (N.le_succ_diag_r offset))
+                    (eq_sym Heqtail30)).
+clear IHe20.
+destruct Stmt.interpret_stmt as ((world30', mem30'), result30').
+remember (fix
+      interpret_expr_list (world0 : world_state) (loc : string_map uint256) 
+                          (e : list AST.expr)
+                          (CallOk : FSet.is_subset (L20.Callset.expr_list_callset e)
+                                      (L20.Callset.decl_callset (fun_decl fc)) = true) {struct e} :
+        world_state * expr_result (list uint256) :=
+        match e as e' return (e = e' -> world_state * expr_result (list uint256)) with
+        | nil => fun _ : e = nil => (world0, ExprSuccess nil)
+        | (h0 :: t)%list =>
+            fun E : e = (h0 :: t)%list =>
+            let (world', result_h) :=
+              L20.Expr.interpret_expr Ebound fc do_call_20 builtins world0 loc h0
+                (L20.Callset.callset_descend_head E CallOk) in
+            match result_h with
+            | ExprSuccess x =>
+                let (world'', result_t) :=
+                  interpret_expr_list world' loc t (L20.Callset.callset_descend_tail E CallOk) in
+                (world'',
+                match result_t with
+                | ExprSuccess y => ExprSuccess (x :: y)%list
+                | ExprAbort _ => result_t
+                end)
+            | ExprAbort ab => (world', ExprAbort ab)
+            end
+        end eq_refl) as interpret_expr_list.
+destruct (interpret_expr_list world30 locmap e20
+            (L20.Callset.callset_descend_tail eq_refl CallOk20))
+  as (world20', result20').
+destruct result20', result30'; try easy.
+
+(* tail computation is finished *)
+destruct IH as (_, (IH_world, (IH_agree, (IH_len, IH_value)))).
+split. { trivial. }
+split. { exact IH_world. }
+clear translate_expr_list Heqtranslate_expr_list ExprOk TailOk Heqhead30 Heqtail30.
+split.
+{
+  unfold mem_agree in *.
+  intros n L NE.
+  rewrite (H_agree n (N.lt_trans _ _ _ L (N.lt_succ_diag_r offset)) NE).
+  assert (NE' := N.lt_trans _ _ _ L (N.lt_succ_diag_r offset)).
+  apply (IH_agree n NE' (N.lt_neq _ _ NE')).
+}
+split. { cbn. now rewrite IH_len. }
+intro i.
+destruct i; cbn.
+{
+  intro Foo. clear Foo.
+  f_equal.
+  rewrite N.add_0_r.
+  apply IH_agree. { apply N.lt_succ_diag_r. }
+  apply N.lt_neq. apply N.lt_succ_diag_r.
+}
+intro L.
+apply lt_S_n in L.
+rewrite (IH_value i L).
+f_equal. f_equal.
+lia.
+Qed.
+
+(* XXX move *)
+Lemma list_eq_by_items {T: Type} (a b: list T)
+                       (Ok: forall i: nat,
+                                 List.nth_error a i
+                                  =
+                                 List.nth_error b i):
+  a = b.
+Proof.
+revert b Ok. induction a as [|ha]; intros; assert (Ok0 := Ok 0); cbn in *.
+{ now destruct b. }
+destruct b as [|hb]. { easy. }
+inversion Ok0. subst hb. f_equal.
+apply IHa. intro i.
+assert (OkSi := Ok (S i)).
+apply OkSi.
+Qed.
+
+Lemma interpret_translated_expr {C: VyperConfig}
+                                {bigger_call_depth_bound smaller_call_depth_bound: nat}
+                                (Ebound: bigger_call_depth_bound = S smaller_call_depth_bound)
+                                {cd20: L20.Descend.calldag}
+                                (builtins: string -> option builtin)
+                                (fc: fun_ctx cd20 bigger_call_depth_bound)
+                                {cd30: L30.Descend.calldag}
+                                (ok: translate_calldag cd20 = inr cd30)
+                                {do_call_20: forall
+                                      (fc': fun_ctx cd20 smaller_call_depth_bound)
+                                      (world: world_state)
+                                      (arg_values: list uint256),
+                                    world_state * expr_result uint256}
+                                {do_call_30: forall
+                                      (fc': fun_ctx cd30 smaller_call_depth_bound)
+                                      (world: world_state)
+                                      (arg_values: list uint256),
+                                    world_state * expr_result uint256}
+                                (DoCallOk: forall fc' world arg_values,
+                                             do_call_30 (translate_fun_ctx fc' ok) world arg_values
+                                              =
+                                             do_call_20 fc' world arg_values)
+                                (world: world_state)
+                                (locmap: string_map uint256)
+                                (locmem: memory)
+                                {e20: L20.AST.expr}
+                                {s30: L30.AST.stmt}
+                                (varmap: string_map N)
+                                (dst offset: N)
+                                (Agree: VarsAgree varmap locmap locmem)
+                                (Bound: VarsBound varmap dst)
+                                (OffsetOk: (dst < offset)%N)
+                                (ExprOk: translate_expr varmap dst offset e20 = inr s30)
+                                (CallOk30: let _ := string_set_impl in 
+                                   FSet.is_subset (L30.Callset.stmt_callset s30)
+                                                  (L30.Callset.decl_callset
+                                                     (fun_decl
+                                                       (translate_fun_ctx fc ok)))
+                                   = true)
+                                (CallOk20: let _ := string_set_impl in 
+                                   FSet.is_subset (L20.Callset.expr_callset e20)
+                                                  (L20.Callset.decl_callset
+                                                    (fun_decl fc))
+                                   = true):
+   let _ := string_map_impl in
+   let _ := memory_impl in
+   let '(world30, mem30, result30) := L30.Stmt.interpret_stmt Ebound (translate_fun_ctx fc ok)
+                                                              do_call_30 builtins
+                                                              world locmem s30 CallOk30
+   in let '(world20, result20) := L20.Expr.interpret_expr Ebound fc do_call_20 builtins
+                                                          world locmap e20 CallOk20
+   in match result20 with
+      | ExprSuccess value20 => result30 = StmtSuccess
+                                /\
+                               world30 = world20
+                                /\
+                               mem_agree offset dst locmem mem30
+                                /\
+                               OpenArray.get mem30 dst = value20
+      | ExprAbort abort => result30 = StmtAbort abort
+      end.
+Proof.
+revert world locmem dst offset Agree Bound OffsetOk s30 ExprOk CallOk30.
+induction e20 using L20.AST.expr_ind'; intros; cbn in ExprOk.
+{ (* Const *)
+  inversion ExprOk. subst.
+  split. { trivial. }
+  split. { trivial. }
+  split.
+  {
+    unfold mem_agree. intros n L NE.
+    rewrite OpenArray.put_ok.
+    enough (F: (dst =? n)%N = false) by now rewrite F.
+    apply N.eqb_neq. intro E. symmetry in E. tauto.
+  }
+  now rewrite OpenArray.put_same.
+}
+{ (* LocalVar *)
+  assert (A := Agree name).
+  unfold map_lookup in *.
+  remember (Map.lookup locmap name) as look_locmap. destruct look_locmap as [value | ].
+  2:{ now destruct (Map.lookup varmap name). }
+  (* the variable is found *)
+  destruct (Map.lookup varmap name). 2:{ contradiction. }
+  inversion ExprOk. subst s30. cbn.
+  unfold map_lookup.
+  rewrite<- Heqlook_locmap.
+  split. { trivial. }
+  split. { trivial. }
+  split.
+  {
+    unfold mem_agree. intros k L NE.
+    rewrite OpenArray.put_ok.
+    enough (F: (dst =? k)%N = false) by now rewrite F.
+    apply N.eqb_neq. intro E. symmetry in E. tauto.
+  }
+  now rewrite OpenArray.put_same.
+}
+{ (* StorageVar *)
+  inversion ExprOk. subst s30. clear ExprOk.
+  cbn.
+  unfold L20.Expr.storage_var_is_declared.
+  assert (D := translate_fun_ctx_declmap fc ok name).
+  destruct (cd_declmap cd20 name) as [vardecl20 | ];
+    destruct (cd_declmap cd30 name) as [vardecl30 | ]; try discriminate.
+  2:easy.
+  destruct vardecl20; cbn in D.
+  {
+    inversion D. subst vardecl30.
+    split. { trivial. }
+    split. { trivial. }
+    split.
+    {
+      unfold mem_agree. intros n L NE.
+      rewrite OpenArray.put_ok.
+      enough (F: (dst =? n)%N = false) by now rewrite F.
+      apply N.eqb_neq. intro E. symmetry in E. tauto.
+    }
+    apply OpenArray.put_same.
+  }
+  destruct make_varmap. { discriminate. }
+  destruct translate_stmt. { discriminate. }
+  inversion D. subst vardecl30.
+  easy.
+}
+{ (* UnOp *)
+  remember (translate_expr varmap dst offset e20) as t.
+  destruct t. { discriminate. }
+  inversion ExprOk. subst s30. cbn. clear ExprOk.
+  assert (IH := IHe20 (L20.Callset.callset_descend_unop eq_refl CallOk20) 
+                      world locmem dst offset Agree Bound OffsetOk s0 (eq_sym Heqt)
+                      (L30.Callset.callset_descend_semicolon_left eq_refl CallOk30)).
+  cbn in IH.
+  destruct L30.Stmt.interpret_stmt as ((world30, mem30), result30).
+  destruct L20.Expr.interpret_expr as (world20, result20).
+  destruct result20, result30; try destruct IH as (I_result, (I_world, (I_agree, I_dst))); 
+    try easy.
+  (* both computations are successful *)
+  subst value.
+  destruct interpret_unop. 2:{ trivial. }
+  split. { trivial. }
+  split. { trivial. }
+  split.
+  {
+    unfold mem_agree in *. intros n L NE.
+    rewrite OpenArray.put_ok.
+    assert (A := I_agree n L NE).
+    enough (F: (dst =? n)%N = false) by now rewrite F.
+    apply N.eqb_neq. intro E. symmetry in E. tauto.
+  }
+  apply OpenArray.put_same.
+}
+{ (* BinOp *)
+  remember (translate_expr varmap dst offset e20_1) as t_1.
+  destruct t_1. { discriminate. }
+  remember (translate_expr varmap offset (N.succ offset) e20_2) as t_2. 
+  destruct t_2. { discriminate. }
+  inversion ExprOk. subst s30. cbn. clear ExprOk.
+  assert (IH_1 := IHe20_1 (L20.Callset.callset_descend_binop_left eq_refl CallOk20)
+                          world locmem dst offset Agree Bound OffsetOk s0 (eq_sym Heqt_1)
+                          (L30.Callset.callset_descend_semicolon_left eq_refl
+                            (L30.Callset.callset_descend_semicolon_left eq_refl CallOk30))).
+  assert (Bound2: VarsBound varmap offset).
+  {
+    apply (vars_bound_loosen Bound).
+    apply N.lt_le_incl.
+    assumption.
+  }
+  cbn in IH_1. clear IHe20_1.
+  destruct L30.Stmt.interpret_stmt as ((world30_1, mem30_1), result30_1).
+  destruct L20.Expr.interpret_expr as (world20_1, result20_1).
+  destruct result20_1, result30_1;
+    try destruct IH_1 as (I1_result, (I1_world, (I1_agree, I1_dst)));
+    try easy.
+  (* both computations of the left operand are successful *)
+  subst world20_1 value.
+  assert (IH_2 := IHe20_2 (L20.Callset.callset_descend_binop_right eq_refl CallOk20)
+                          world30_1 mem30_1 offset (N.succ offset)
+                          (vars_agree_if_mem_agree _ _ _ _ Agree _ _ Bound OffsetOk I1_agree)
+                          Bound2
+                          (N.lt_succ_diag_r offset)
+                          s1 (eq_sym Heqt_2)
+                          (L30.Callset.callset_descend_semicolon_right eq_refl
+                            (L30.Callset.callset_descend_semicolon_left eq_refl CallOk30))).
+  cbn in IH_2. clear IHe20_2.
+  destruct L30.Stmt.interpret_stmt as ((world30_2, mem30_2), result30_2).
+  destruct L20.Expr.interpret_expr as (world20_2, result20_2).
+  destruct result20_2, result30_2;
+    try destruct IH_2 as (I2_result, (I2_world, (I2_agree, I2_dst)));
+    try easy.
+  (* both computations of the right operand are successful *)
+  subst world20_2 value.
+  assert (A: OpenArray.get mem30_1 dst = OpenArray.get mem30_2 dst).
+  {
+    apply I2_agree.
+    { apply (N.lt_trans _ _ _ OffsetOk (N.lt_succ_diag_r _)). }
+    apply (N.lt_neq _ _ OffsetOk).
+  }
+  unfold m in *.
+  rewrite A.
+  destruct interpret_binop. 2:{ trivial. }
+  split. { trivial. }
+  split. { trivial. }
+  split.
+  {
+    unfold mem_agree in *. intros n L NE.
+    rewrite OpenArray.put_ok.
+    assert (F: (dst =? n)%N = false).
+    { apply N.eqb_neq. intro E. symmetry in E. tauto. }
+    rewrite F.
+    rewrite I1_agree by assumption.
+    apply I2_agree.
+    { apply (N.lt_trans _ _ _ L (N.lt_succ_diag_r _)). }
+    apply (N.lt_neq _ _ L).
+  }
+  apply OpenArray.put_same.
+}
+{ (* IfThenElse *)
+  remember (translate_expr varmap dst offset e20_1) as t_cond.
+  destruct t_cond. { discriminate. }
+  remember (translate_expr varmap dst offset e20_2) as t_yes.
+  destruct t_yes. { discriminate. }
+  remember (translate_expr varmap dst offset e20_3) as t_no.
+  destruct t_no. { discriminate. }
+  inversion ExprOk. subst s30. cbn. clear ExprOk.
+  assert (IH_1 := IHe20_1 (L20.Callset.callset_descend_if_cond eq_refl CallOk20)
+                          world locmem dst offset Agree Bound OffsetOk s0 (eq_sym Heqt_cond)
+                          (L30.Callset.callset_descend_semicolon_left eq_refl CallOk30)).
+  cbn in IH_1. clear IHe20_1.
+  destruct L30.Stmt.interpret_stmt as ((world30_1, mem30_1), result30_1).
+  destruct L20.Expr.interpret_expr as (world20_1, result20_1).
+  destruct result20_1, result30_1;
+    try destruct IH_1 as (I1_result, (I1_world, (I1_agree, I1_dst)));
+    try easy.
+  (* cond computation succeeded *)
+  subst value.
+  destruct (Z_of_uint256 (OpenArray.get mem30_1 dst) =? 0)%Z.
+  {
+    (* else *)
+    clear IHe20_2. subst world20_1.
+    assert (IH_3 := IHe20_3 (L20.Callset.callset_descend_if_else eq_refl CallOk20)
+                        world30_1 mem30_1 dst offset
+                        (vars_agree_if_mem_agree _ _ _ _ Agree _ _ Bound OffsetOk I1_agree)
+                        Bound OffsetOk s2 (eq_sym Heqt_no)
+                        (L30.Callset.callset_descend_stmt_if_else eq_refl
+                          (L30.Callset.callset_descend_semicolon_right eq_refl CallOk30))).
+    cbn in IH_3. clear IHe20_3.
+    destruct L30.Stmt.interpret_stmt as ((world30_3, mem30_3), result30_3).
+    destruct L20.Expr.interpret_expr as (world20_3, result20_3).
+    destruct result20_3, result30_3;
+      try destruct IH_3 as (I3_result, (I3_world, (I3_agree, I3_dst)));
+      try easy.
+    (* else branch computation succeeded *)
+    split. { trivial. }
+    split. { trivial. }
+    split. 2:assumption.
+    unfold mem_agree in *. intros.
+    rewrite I1_agree by assumption.
+    apply I3_agree; assumption.
+  }
+  (* then *)
+  clear IHe20_3. subst world20_1.
+  assert (IH_2 := IHe20_2 (L20.Callset.callset_descend_if_then eq_refl CallOk20)
+                      world30_1 mem30_1 dst offset
+                      (vars_agree_if_mem_agree _ _ _ _ Agree _ _ Bound OffsetOk I1_agree)
+                      Bound OffsetOk s1 (eq_sym Heqt_yes)
+                      (L30.Callset.callset_descend_stmt_if_then eq_refl
+                        (L30.Callset.callset_descend_semicolon_right eq_refl CallOk30))).
+  cbn in IH_2. clear IHe20_2.
+  destruct L30.Stmt.interpret_stmt as ((world30_2, mem30_2), result30_2).
+  destruct L20.Expr.interpret_expr as (world20_2, result20_2).
+  destruct result20_2, result30_2;
+    try destruct IH_2 as (I2_result, (I2_world, (I2_agree, I2_dst)));
+    try easy.
+  (* else branch computation succeeded *)
+  split. { trivial. }
+  split. { trivial. }
+  split. 2:assumption.
+  unfold mem_agree in *. intros.
+  rewrite I1_agree by assumption.
+  apply I2_agree; assumption.
+}
+{ (* LogicalAnd *)
+  remember (translate_expr varmap dst offset e20_1) as t_1.
+  destruct t_1. { discriminate. }
+  remember (translate_expr varmap dst offset e20_2) as t_2.
+  destruct t_2. { discriminate. }
+  inversion ExprOk. subst s30. cbn. clear ExprOk.
+  assert (IH_1 := IHe20_1 (L20.Callset.callset_descend_and_left eq_refl CallOk20)
+                        world locmem dst offset Agree Bound OffsetOk s0 (eq_sym Heqt_1)
+                        (L30.Callset.callset_descend_semicolon_left eq_refl CallOk30)).
+  cbn in IH_1. clear IHe20_1.
+  destruct L30.Stmt.interpret_stmt as ((world30_1, mem30_1), result30_1).
+  destruct L20.Expr.interpret_expr as (world20_1, result20_1).
+  destruct result20_1, result30_1;
+    try destruct IH_1 as (I1_result, (I1_world, (I1_agree, I1_dst)));
+    try easy.
+  (* left operand computation succeeded *)
+  subst value.
+  destruct (Z_of_uint256 (OpenArray.get mem30_1 dst) =? 0)%Z.
+  {
+    split. { trivial. }
+    split. { trivial. }
+    split. { assumption. }
+    trivial.
+  }
+  (* we'll compute the right operand *)
+  subst world20_1.
+  assert (IH_2 := IHe20_2 (L20.Callset.callset_descend_and_right eq_refl CallOk20)
+                      world30_1 mem30_1 dst offset
+                      (vars_agree_if_mem_agree _ _ _ _ Agree _ _ Bound OffsetOk I1_agree)
+                      Bound OffsetOk s1 (eq_sym Heqt_2)
+                      (L30.Callset.callset_descend_stmt_if_then eq_refl
+                        (L30.Callset.callset_descend_semicolon_right eq_refl CallOk30))).
+  cbn in IH_2. clear IHe20_2.
+  destruct L30.Stmt.interpret_stmt as ((world30_2, mem30_2), result30_2).
+  destruct L20.Expr.interpret_expr as (world20_2, result20_2).
+  destruct result20_2, result30_2;
+    try destruct IH_2 as (I2_result, (I2_world, (I2_agree, I2_dst)));
+    try easy.
+  (* right operand computation succeeded *)
+  split. { trivial. }
+  split. { trivial. }
+  split. 2:assumption.
+  unfold mem_agree in *. intros.
+  rewrite I1_agree by assumption.
+  apply I2_agree; assumption.
+}
+{ (* LogicalOr *)
+  remember (translate_expr varmap dst offset e20_1) as t_1.
+  destruct t_1. { discriminate. }
+  remember (translate_expr varmap dst offset e20_2) as t_2.
+  destruct t_2. { discriminate. }
+  inversion ExprOk. subst s30. cbn. clear ExprOk.
+  assert (IH_1 := IHe20_1 (L20.Callset.callset_descend_or_left eq_refl CallOk20)
+                        world locmem dst offset Agree Bound OffsetOk s0 (eq_sym Heqt_1)
+                        (L30.Callset.callset_descend_semicolon_left eq_refl CallOk30)).
+  cbn in IH_1. clear IHe20_1.
+  destruct L30.Stmt.interpret_stmt as ((world30_1, mem30_1), result30_1).
+  destruct L20.Expr.interpret_expr as (world20_1, result20_1).
+  destruct result20_1, result30_1;
+    try destruct IH_1 as (I1_result, (I1_world, (I1_agree, I1_dst)));
+    try easy.
+  (* left operand computation succeeded *)
+  subst value.
+  destruct (Z_of_uint256 (OpenArray.get mem30_1 dst) =? 0)%Z.
+  2:{
+    split. { trivial. }
+    split. { trivial. }
+    split. { assumption. }
+    trivial.
+  }
+  (* we'll compute the right operand *)
+  subst world20_1.
+  assert (IH_2 := IHe20_2 (L20.Callset.callset_descend_or_right eq_refl CallOk20)
+                      world30_1 mem30_1 dst offset
+                      (vars_agree_if_mem_agree _ _ _ _ Agree _ _ Bound OffsetOk I1_agree)
+                      Bound OffsetOk s1 (eq_sym Heqt_2)
+                      (L30.Callset.callset_descend_stmt_if_else eq_refl
+                        (L30.Callset.callset_descend_semicolon_right eq_refl CallOk30))).
+  cbn in IH_2. clear IHe20_2.
+  destruct L30.Stmt.interpret_stmt as ((world30_2, mem30_2), result30_2).
+  destruct L20.Expr.interpret_expr as (world20_2, result20_2).
+  destruct result20_2, result30_2;
+    try destruct IH_2 as (I2_result, (I2_world, (I2_agree, I2_dst)));
+    try easy.
+  (* right operand computation succeeded *)
+  split. { trivial. }
+  split. { trivial. }
+  split. 2:assumption.
+  unfold mem_agree in *. intros.
+  rewrite I1_agree by assumption.
+  apply I2_agree; assumption.
+}
+{ (* PrivateCall *)
+  remember (_ varmap offset args) as translated_args.
+  destruct translated_args. { discriminate. }
+  inversion ExprOk. subst s30. clear ExprOk. clear s. unfold m. clear m.
+  assert (ArgsOk := weak_interpret_translated_exprs Ebound builtins fc ok DoCallOk
+                    world locmap locmem varmap offset Agree 
+                    (vars_bound_loosen Bound (N.lt_le_incl _ _ OffsetOk))
+                    (eq_sym Heqtranslated_args)
+                    (L30.Callset.callset_descend_semicolon_left eq_refl CallOk30)
+                    (L20.Callset.callset_descend_args eq_refl CallOk20)
+                    H).
+  cbn in ArgsOk. clear H Heqtranslated_args. cbn.
+  destruct L30.Stmt.interpret_stmt as ((world30_args, mem30_args), result30_args).
+  remember (fix
+      interpret_expr_list (world0 : world_state) (loc : string_map uint256) 
+                          (e : list AST.expr)
+                          (CallOk : FSet.is_subset (L20.Callset.expr_list_callset e)
+                                      (L20.Callset.decl_callset (fun_decl fc)) = true) {struct e} :
+        world_state * expr_result (list uint256) :=
+        match e as e' return (e = e' -> world_state * expr_result (list uint256)) with
+        | nil => fun _ : e = nil => (world0, ExprSuccess nil)
+        | (h0 :: t)%list =>
+            fun E : e = (h0 :: t)%list =>
+            let (world', result_h) :=
+              L20.Expr.interpret_expr Ebound fc do_call_20 builtins world0 loc h0
+                (L20.Callset.callset_descend_head E CallOk) in
+            match result_h with
+            | ExprSuccess x =>
+                let (world'', result_t) :=
+                  interpret_expr_list world' loc t (L20.Callset.callset_descend_tail E CallOk) in
+                (world'',
+                match result_t with
+                | ExprSuccess y => ExprSuccess (x :: y)%list
+                | ExprAbort _ => result_t
+                end)
+            | ExprAbort ab => (world', ExprAbort ab)
+            end
+        end eq_refl) as interpret_expr_list.
+  destruct interpret_expr_list as (world20_args, result20_args).
+  destruct result20_args, result30_args; try easy.
+  destruct ArgsOk as (_, (Args_world, (Args_agree, (Args_len, Args_dst)))).
+  (* args computation has succeeded *)
+
+  assert (D: L30.Descend.fun_ctx_descend (translate_fun_ctx fc ok)
+              (Callset.callset_descend_small_stmt eq_refl
+                (Callset.callset_descend_semicolon_right eq_refl CallOk30))
+              Ebound eq_refl
+              =
+             match L20.Descend.fun_ctx_descend fc CallOk20 Ebound eq_refl with
+             | Some ctx => Some (translate_fun_ctx ctx ok)
+             | None => None
+             end).
+  {
+    (* This follows fun_ctx_descend_irrel. *)
+    unfold L20.Descend.fun_ctx_descend.
+    unfold L30.Descend.fun_ctx_descend.
+    assert (InnerOk: forall (d1: L20.AST.decl)
+                            (Edecl1: cd_declmap cd20 name = Some d1)
+                            (d2: L30.AST.decl)
+                            (Edecl2: cd_declmap cd30 name = Some d2),
+                   L30.Descend.fun_ctx_descend_inner (translate_fun_ctx fc ok)
+                      (Callset.callset_descend_small_stmt eq_refl
+                        (Callset.callset_descend_semicolon_right eq_refl CallOk30))
+                      Ebound eq_refl Edecl2
+                    =
+                   match L20.Descend.fun_ctx_descend_inner fc CallOk20 Ebound eq_refl Edecl1 with
+                   | Some ctx20 => Some (translate_fun_ctx ctx20 ok)
+                   | None => None
+                   end).
+    {
+      intros.
+      unfold L20.Descend.fun_ctx_descend_inner.
+      unfold L30.Descend.fun_ctx_descend_inner.
+      remember (fun (depth: nat) (Edepth: cd_depthmap cd30 name = Some depth) =>
+          Some
+            {|
+            fun_name := name;
+            fun_depth := depth;
+            fun_depth_ok := Edepth;
+            fun_decl := d2;
+            fun_decl_ok := Edecl2;
+            fun_bound_ok := L30.Descend.call_descend' (translate_fun_ctx fc ok)
+                        (Callset.callset_descend_small_stmt eq_refl
+                           (Callset.callset_descend_semicolon_right eq_refl CallOk30)) Ebound eq_refl
+                              Edecl2 Edepth |})
+        as some_branch_l.
+      remember (fun Edepth : cd_depthmap cd30 name = None =>
+                  False_rect (option (fun_ctx cd30 smaller_call_depth_bound))
+                             (Descend.fun_ctx_descend_helper Edecl2 Edepth))
+        as none_branch_l.
+      remember (fun (depth: nat) (Edepth: cd_depthmap cd20 name = Some depth) =>
+        Some
+          {|
+          fun_name := name;
+          fun_depth := depth;
+          fun_depth_ok := Edepth;
+          fun_decl := d1;
+          fun_decl_ok := Edecl1;
+          fun_bound_ok := L20.Descend.call_descend' fc CallOk20 Ebound eq_refl Edecl1 Edepth |})
+        as some_branch_r.
+      remember (fun Edepth : cd_depthmap cd20 name = None =>
+                    False_rect (option (fun_ctx cd20 smaller_call_depth_bound))
+                      (L20.Descend.fun_ctx_descend_helper Edecl1 Edepth))
+        as none_branch_r.
+      assert (NoneOkL: forall (Edepth: cd_depthmap cd30 name = None),
+                         none_branch_l Edepth = None).
+      { intro. exfalso. exact (L30.Descend.fun_ctx_descend_helper Edecl2 Edepth). }
+      assert (NoneOkR: forall (Edepth: cd_depthmap cd20 name = None),
+                         none_branch_r Edepth = None).
+      { intro. exfalso. exact (L20.Descend.fun_ctx_descend_helper Edecl1 Edepth). }
+      clear Heqnone_branch_l Heqnone_branch_r.
+      revert none_branch_l none_branch_r NoneOkL NoneOkR.
+      assert (SomeBranchOk: forall (depth: nat)
+                                   (Edepth1: cd_depthmap cd20 name = Some depth)
+                                   (Edepth2: cd_depthmap cd30 name = Some depth),
+                     some_branch_l depth Edepth2 
+                      =
+                     match some_branch_r depth Edepth1 with
+                     | Some ctx20 => Some (translate_fun_ctx ctx20 ok)
+                     | None => None
+                     end).
+      {
+        intros. subst. unfold translate_fun_ctx. cbn.
+        f_equal.
+        assert (D: d2 = cached_translated_decl
+                {|
+                fun_name := name;
+                fun_depth := depth;
+                fun_depth_ok := Edepth1;
+                fun_decl := d1;
+                fun_decl_ok := Edecl1;
+                fun_bound_ok := L20.Descend.call_descend' fc CallOk20 eq_refl eq_refl Edecl1 Edepth1 |}
+                ok).
+        {
+          unfold cached_translated_decl. cbn.
+          remember (FunCtx.translate_fun_ctx_fun_decl_helper _ ok) as Bad. clear HeqBad.
+          cbn in Bad. revert Bad.
+          destruct (cd_declmap cd30 name). { now inversion Edecl2. }
+          intro Bad. discriminate.
+        }
+        subst. f_equal; apply PropExtensionality.proof_irrelevance.
+      } (* SomeBranchOk *)
+      clear Heqsome_branch_l Heqsome_branch_r
+            CallOk20 CallOk30 Edecl1 Edecl2 d1 d2 args value DoCallOk
+            do_call_20 do_call_30 Heqinterpret_expr_list Args_dst Args_len.
+      revert some_branch_l some_branch_r SomeBranchOk.
+      rewrite (translate_fun_ctx_depthmap fc ok name).
+      destruct (cd_depthmap cd20 name); intros. { apply SomeBranchOk. }
+      rewrite (NoneOkL eq_refl).
+      rewrite (NoneOkR eq_refl).
+      trivial.
+    } (* InnerOk *)
+    remember L30.Descend.fun_ctx_descend_inner as inner30. clear Heqinner30.
+    remember L20.Descend.fun_ctx_descend_inner as inner20. clear Heqinner20.
+    subst.
+    remember (cd_declmap cd20 name) as maybe_d20.
+    remember (fun d0 (Edecl : cd_declmap cd30 name = Some d0) =>
+                    inner30 (translate_fun_ctx fc ok)
+                      (Callset.callset_descend_small_stmt eq_refl
+                         (Callset.callset_descend_semicolon_right eq_refl CallOk30)) eq_refl name dst offset
+                      (N.of_nat (Datatypes.length args)) eq_refl d0 Edecl)
+      as some_branch.
+    destruct maybe_d20.
+    {
+      assert (SomeBranchOk: forall (d30: L30.AST.decl)
+                                   (Edecl: cd_declmap cd30 name = Some d30),
+                     some_branch d30 Edecl
+                      =
+                     match inner20 fc CallOk20 eq_refl eq_refl d eq_refl with
+                     | Some ctx => Some (translate_fun_ctx ctx ok)
+                     | None => None
+                     end).
+      { apply InnerOk. }
+      clear Heqsome_branch.
+      remember (cd_declmap cd30 name) as maybe_d30.
+      destruct maybe_d30. { apply SomeBranchOk. }
+      assert (T := translate_fun_ctx_declmap fc ok name).
+      rewrite<- Heqmaybe_d20 in T. rewrite<- Heqmaybe_d30 in T.
+      discriminate.
+    }
+    assert (SomeBranchOk: forall (d30: L30.AST.decl)
+                             (Edecl: cd_declmap cd30 name = Some d30),
+               some_branch d30 Edecl
+                =
+               None).
+    {
+      intros.
+      assert (T := translate_fun_ctx_declmap fc ok name).
+      rewrite<- Heqmaybe_d20 in T. rewrite Edecl in T.
+      discriminate.
+    }
+    clear Heqsome_branch.
+    now destruct (cd_declmap cd30 name).
+  } (* D *)
+  assert (R: (@Callset.callset_descend_small_stmt C
+         (@AST.SmallStmt C
+            (@AST.PrivateCall C dst name offset (N.of_nat (@Datatypes.length (@AST.expr C) args))))
+         (@AST.PrivateCall C dst name offset (N.of_nat (@Datatypes.length (@AST.expr C) args)))
+         (@Callset.decl_callset C
+            (@fun_decl C (@AST.decl C) (@Callset.decl_callset C) cd30 bigger_call_depth_bound
+               (@translate_fun_ctx C bigger_call_depth_bound cd20 fc cd30 ok)))
+         (@eq_refl (@AST.stmt C)
+            (@AST.SmallStmt C
+               (@AST.PrivateCall C dst name offset (N.of_nat (@Datatypes.length (@AST.expr C) args)))))
+         (@Callset.callset_descend_semicolon_right C s0
+            (@AST.SmallStmt C
+               (@AST.PrivateCall C dst name offset (N.of_nat (@Datatypes.length (@AST.expr C) args))))
+            (@AST.Semicolon C s0
+               (@AST.SmallStmt C
+                  (@AST.PrivateCall C dst name offset
+                     (N.of_nat (@Datatypes.length (@AST.expr C) args)))))
+            (@Callset.decl_callset C
+               (@fun_decl C (@AST.decl C) (@Callset.decl_callset C) cd30 bigger_call_depth_bound
+                  (@translate_fun_ctx C bigger_call_depth_bound cd20 fc cd30 ok)))
+            (@eq_refl (@AST.stmt C)
+               (@AST.Semicolon C s0
+                  (@AST.SmallStmt C
+                     (@AST.PrivateCall C dst name offset
+                        (N.of_nat (@Datatypes.length (@AST.expr C) args)))))) CallOk30))
+            =
+         (@Callset.callset_descend_small_stmt C
+            (@AST.SmallStmt C
+               (@AST.PrivateCall C dst name offset (N.of_nat (@Datatypes.length (@AST.expr C) args))))
+            (@AST.PrivateCall C dst name offset (N.of_nat (@Datatypes.length (@AST.expr C) args)))
+            (@Callset.decl_callset C (@cached_translated_decl C bigger_call_depth_bound cd20 fc cd30 ok))
+            (@eq_refl (@AST.stmt C)
+               (@AST.SmallStmt C
+                  (@AST.PrivateCall C dst name offset (N.of_nat (@Datatypes.length (@AST.expr C) args)))))
+            (@Callset.callset_descend_semicolon_right C s0
+               (@AST.SmallStmt C
+                  (@AST.PrivateCall C dst name offset (N.of_nat (@Datatypes.length (@AST.expr C) args))))
+               (@AST.Semicolon C s0
+                  (@AST.SmallStmt C
+                     (@AST.PrivateCall C dst name offset (N.of_nat (@Datatypes.length (@AST.expr C) args)))))
+               (@Callset.decl_callset C
+                  (@cached_translated_decl C bigger_call_depth_bound cd20 fc cd30 ok))
+               (@eq_refl (@AST.stmt C)
+                  (@AST.Semicolon C s0
+                     (@AST.SmallStmt C
+                        (@AST.PrivateCall C dst name offset
+                           (N.of_nat (@Datatypes.length (@AST.expr C) args)))))) CallOk30))).
+  { apply PropExtensionality.proof_irrelevance. }
+  rewrite<- R. clear R.
+  rewrite D. clear D.
+  destruct (L20.Descend.fun_ctx_descend fc CallOk20 Ebound eq_refl). 2:easy.
+  rewrite DoCallOk. rewrite Args_world.
+
+  assert (V: let _ := memory_impl in
+             OpenArray.view mem30_args offset (N.of_nat (Datatypes.length args)) = value).
+  {
+    clear interpret_expr_list Heqinterpret_expr_list CallOk30 world30_args world20_args
+          f Args_world Args_agree CallOk20 dst OffsetOk Bound.
+    apply list_eq_by_items.
+    intro i.
+    assert (OkV := let _ := memory_impl in
+                   OpenArray.view_ok mem30_args offset (N.of_nat (Datatypes.length args))).
+    assert (K := Nat.lt_ge_cases i (List.length args)).
+    case K; clear K; intro K.
+    {
+      rewrite (Args_dst i K).
+      rewrite<- (OkV (N.of_nat i)).
+      { now rewrite Nat2N.id. }
+      lia.
+    }
+    assert (L := K).
+    rewrite<- Args_len in L.
+    rewrite<- List.nth_error_None in L. rewrite L.
+    apply List.nth_error_None.
+    rewrite OpenArray.view_len.
+    lia.
+  } (* V *)
+  rewrite V.
+  destruct (do_call_20 f world20_args value).
+  destruct e as [value20|]. 2:easy.
+  split. { trivial. }
+  split. { trivial. }
+  split. 2:apply OpenArray.put_same.
+  unfold mem_agree in *.
+  intros n L NE.
+  rewrite (Args_agree n L (N.lt_neq _ _ L)).
+  rewrite OpenArray.put_ok.
+  enough (F: (dst =? n)%N = false) by now rewrite F.
+  rewrite N.eqb_sym.
+  apply N.eqb_neq.
+  exact NE.
+}
+(* BuiltinCall *)
+remember (_ varmap offset args) as translated_args.
+destruct translated_args. { discriminate. }
+inversion ExprOk. subst s30. clear ExprOk. clear s. unfold m. clear m.
+assert (ArgsOk := weak_interpret_translated_exprs Ebound builtins fc ok DoCallOk
+                  world locmap locmem varmap offset Agree 
+                  (vars_bound_loosen Bound (N.lt_le_incl _ _ OffsetOk))
+                  (eq_sym Heqtranslated_args)
+                  (L30.Callset.callset_descend_semicolon_left eq_refl CallOk30)
+                  (L20.Callset.callset_descend_builtin_args eq_refl CallOk20)
+                  H).
+cbn in ArgsOk. clear H Heqtranslated_args. cbn.
+destruct L30.Stmt.interpret_stmt as ((world30_args, mem30_args), result30_args).
+remember (fix
+    interpret_expr_list (world0 : world_state) (loc : string_map uint256) 
+                        (e : list AST.expr)
+                        (CallOk : FSet.is_subset (L20.Callset.expr_list_callset e)
+                                    (L20.Callset.decl_callset (fun_decl fc)) = true) {struct e} :
+      world_state * expr_result (list uint256) :=
+      match e as e' return (e = e' -> world_state * expr_result (list uint256)) with
+      | nil => fun _ : e = nil => (world0, ExprSuccess nil)
+      | (h0 :: t)%list =>
+          fun E : e = (h0 :: t)%list =>
+          let (world', result_h) :=
+            L20.Expr.interpret_expr Ebound fc do_call_20 builtins world0 loc h0
+              (L20.Callset.callset_descend_head E CallOk) in
+          match result_h with
+          | ExprSuccess x =>
+              let (world'', result_t) :=
+                interpret_expr_list world' loc t (L20.Callset.callset_descend_tail E CallOk) in
+              (world'',
+              match result_t with
+              | ExprSuccess y => ExprSuccess (x :: y)%list
+              | ExprAbort _ => result_t
+              end)
+          | ExprAbort ab => (world', ExprAbort ab)
+          end
+      end eq_refl) as interpret_expr_list.
+destruct interpret_expr_list as (world20_args, result20_args).
+destruct result20_args, result30_args; try easy.
+destruct ArgsOk as (_, (Args_world, (Args_agree, (Args_len, Args_dst)))).
+
+assert (V: let _ := memory_impl in
+           OpenArray.view mem30_args offset (N.of_nat (Datatypes.length args)) = value).
+{
+  clear interpret_expr_list Heqinterpret_expr_list CallOk30 world30_args world20_args
+        Args_world Args_agree CallOk20 dst OffsetOk Bound.
+  apply list_eq_by_items.
+  intro i.
+  assert (OkV := let _ := memory_impl in
+                 OpenArray.view_ok mem30_args offset (N.of_nat (Datatypes.length args))).
+  assert (K := Nat.lt_ge_cases i (List.length args)).
+  case K; clear K; intro K.
+  {
+    rewrite (Args_dst i K).
+    rewrite<- (OkV (N.of_nat i)).
+    { now rewrite Nat2N.id. }
+    lia.
+  }
+  assert (L := K).
+  rewrite<- Args_len in L.
+  rewrite<- List.nth_error_None in L. rewrite L.
+  apply List.nth_error_None.
+  rewrite OpenArray.view_len.
+  lia.
+} (* V *)
+
+destruct (builtins name) as [(arity, builtin)|]. 2:easy.
+remember (fun Earity : (arity =? Datatypes.length (OpenArray.view mem30_args offset (N.of_nat (Datatypes.length args)))) = true =>
+   let '(world', call_result) :=
+     call_builtin (OpenArray.view mem30_args offset (N.of_nat (Datatypes.length args))) Earity (builtin world30_args) in
+   match call_result with
+   | ExprSuccess result => (world', OpenArray.put mem30_args dst result, StmtSuccess)
+   | ExprAbort ab => (world', mem30_args, StmtAbort ab)
+   end) as good_branch_30.
+assert (GoodBranch30Ok: let _ := memory_impl in
+         forall Earity: (arity =? Datatypes.length (OpenArray.view mem30_args offset (N.of_nat (Datatypes.length args))) = true),
+           let '(world30, mem30, result30) := good_branch_30 Earity in
+           match
+             (if arity =? Datatypes.length value as arity_ok
+               return ((arity =? Datatypes.length value) = arity_ok -> world_state * expr_result uint256)
+              then
+               fun Earity : (arity =? Datatypes.length value) = true =>
+               call_builtin value Earity (builtin world20_args)
+              else
+               fun _ : (arity =? Datatypes.length value) = false =>
+               (world20_args, expr_error "builtin with wrong arity")) eq_refl
+           with
+           | (world20, ExprSuccess value20) =>
+               result30 = StmtSuccess /\
+               world30 = world20 /\ mem_agree offset dst locmem mem30 /\ OpenArray.get mem30 dst = value20
+           | (world20, ExprAbort abort) => result30 = StmtAbort abort
+           end).
+{
+  cbn. intro Earity. subst good_branch_30.
+  subst world30_args.
+  assert (Earity': (arity =? Datatypes.length value) = true).
+  {
+    rewrite OpenArray.view_len in Earity.
+    rewrite Nat2N.id in Earity.
+    now rewrite Args_len.
+  }
+  replace ((if arity =? Datatypes.length value as arity_ok
+             return ((arity =? Datatypes.length value) = arity_ok -> world_state * expr_result uint256)
+            then fun Earity0 : (arity =? Datatypes.length value) = true =>
+                   call_builtin value Earity0 (builtin world20_args)
+            else
+             fun _ : (arity =? Datatypes.length value) = false =>
+             (world20_args, expr_error "builtin with wrong arity")) eq_refl) 
+  with (call_builtin value Earity' (builtin world20_args)).
+  2:{
+    clear Earity.
+    remember (call_builtin value Earity' (builtin world20_args)) as lhs.
+    remember (fun Earity0 : (arity =? Datatypes.length value) = true =>
+                call_builtin value Earity0 (builtin world20_args)) as good_rhs.
+    assert (E: lhs = good_rhs Earity') by now subst.
+    clear Heqlhs Heqgood_rhs.
+    destruct (arity =? Datatypes.length value).
+    {
+      assert (Earity' = eq_refl). { apply PropExtensionality.proof_irrelevance. }
+      now subst.
+    }
+    discriminate.
+  }
+  revert Earity Earity'.
+  rewrite V.
+  intros.
+  assert (Earity = Earity'). { apply PropExtensionality.proof_irrelevance. }
+  subst Earity'.
+  destruct (call_builtin value Earity (builtin world20_args)).
+  destruct e. 2:easy.
+  split. { trivial. }
+  split. { trivial. }
+  split. 2:apply OpenArray.put_same.
+  unfold mem_agree in *.
+  intros n L NE.
+  rewrite (Args_agree n L (N.lt_neq _ _ L)).
+  rewrite OpenArray.put_ok.
+  enough (Q: (dst =? n)%N = false) by now rewrite Q.
+  rewrite N.eqb_neq. intro H. symmetry in H. tauto.
+}
+clear Heqgood_branch_30.
+remember (arity =? Datatypes.length (OpenArray.view mem30_args offset (N.of_nat (Datatypes.length args))))
+  as arity_ok.
+destruct arity_ok. { apply GoodBranch30Ok. }
+(* arity check failed *)
+assert (F: arity =? Datatypes.length value = false).
+{
+  rewrite OpenArray.view_len in Heqarity_ok.
+  rewrite Nat2N.id in Heqarity_ok.
+  now rewrite Args_len.
+}
+remember (fun Earity : (arity =? Datatypes.length value) = true =>
+            call_builtin value Earity (builtin world20_args)) as good_branch_20.
+clear Heqgood_branch_20.
+destruct (arity =? Datatypes.length value). { discriminate. }
+easy.
+Qed.
